Prove adequacy in a generic manner.

Linker.v
@@ -4,140 +4,9 @@ Require Import Coqlib Coqlib_linker.
 Require Import Maps Maps_linker.
 Require Import Integers Floats Values AST Globalenvs.
 Require Import Errors Behaviors Compiler Smallstep.
+Require Import Language.
 
 Set Implicit Arguments.
-
-Definition external_function_ext :=
-  (external_function * Ctypes.typelist * Ctypes.type * calling_convention)%type.
-
-Definition external_function_ext_eq (ef1 ef2: external_function_ext): {ef1 = ef2} + {ef1 <> ef2}.
-Proof.
-  destruct ef1 as [[[ef1 args1] res1] cc1].
-  destruct ef2 as [[[ef2 args2] res2] cc2].
-  decide equality.
-  { destruct b, c.
-    destruct (bool_dec cc_vararg cc_vararg0); [subst|].
-    { destruct (bool_dec cc_structret cc_structret0); [subst|].
-      { left. auto. }
-      { right. contradict n. inv n. auto. }
-    }
-    { right. contradict n. inv n. auto. }
-  }
-  decide equality.
-  { apply Ctypes.type_eq. }
-  decide equality.
-  { apply Ctypes.typelist_eq. }
-  { apply external_function_eq. }
-Defined.
-
-(** Structures *)
-
-Structure Sig: Type := mkSig {
-  Sig_carrier :> Type;
-  Sig_dec: forall (sig1 sig2:Sig_carrier), {sig1 = sig2} + {sig1 <> sig2}
-}.
-
-Structure F (sigT:Sig): Type := mkF {
-  F_carrier :> Type;
-  F_sig: forall (f:F_carrier), sigT
-}.
-
-Structure EF (sigT:Sig): Type := mkEF {
-  EF_carrier :> Type;
-  EF_dec: forall (ef1 ef2:EF_carrier), {ef1 = ef2} + {ef1 <> ef2};
-  EF_linkable: forall (ef:EF_carrier), bool;
-  EF_sig: forall (ef:EF_carrier), sigT
-}.
-
-Structure Fundef (sigT:Sig) (fT:F sigT) (efT:EF sigT) := mkFundef {
-  Fundef_carrier :> Type;
-  Fundef_dec: forall (fd:Fundef_carrier), fT + efT;
-  Fundef_sig :=
-    fun fd =>
-      match Fundef_dec fd with
-        | inl f => fT.(F_sig) f
-        | inr ef => efT.(EF_sig) ef
-      end
-}.
-
-Structure V: Type := mkV {
-  V_carrier :> Type;
-  V_dec: forall (v1 v2:V_carrier), {v1 = v2} + {v1 <> v2}
-}.
-
-Structure Language: Type := mkLanguage {
-  sigT: Sig;
-  fT: F sigT;
-  efT: EF sigT;
-  fundefT: Fundef fT efT;
-  vT: V;
-
-  globdefT := AST.globdef fundefT vT;
-  progT := AST.program fundefT vT
-}.
-
-(** Canonical Structures *)
-
-Canonical Structure Sig_type: Sig := mkSig Ctypes.type_eq.
-Canonical Structure Sig_signature: Sig := mkSig signature_eq.
-
-Canonical Structure F_C: F Sig_type := mkF Sig_type Csyntax.type_of_function.
-Canonical Structure F_Clight: F Sig_type := mkF Sig_type Clight.type_of_function.
-Canonical Structure F_Csharpminor: F Sig_signature := mkF Sig_signature Csharpminor.fn_sig.
-Canonical Structure F_Cminor: F Sig_signature := mkF Sig_signature Cminor.fn_sig.
-Canonical Structure F_CminorSel: F Sig_signature := mkF Sig_signature CminorSel.fn_sig.
-Canonical Structure F_RTL: F Sig_signature := mkF Sig_signature RTL.fn_sig.
-Canonical Structure F_LTL: F Sig_signature := mkF Sig_signature LTL.fn_sig.
-Canonical Structure F_Linear: F Sig_signature := mkF Sig_signature Linear.fn_sig.
-Canonical Structure F_Mach: F Sig_signature := mkF Sig_signature Mach.fn_sig.
-Canonical Structure F_Asm: F Sig_signature := mkF Sig_signature Asm.fn_sig.
-
-Canonical Structure EF_external_function_ext: EF Sig_type :=
-  mkEF Sig_type
-       external_function_ext_eq
-       (fun ef => match ef with (EF_external _ _, _, _, _) => true | _ => false end)
-       (fun ef => match ef with (_, targs, tres, cc) => Ctypes.Tfunction targs tres cc end).
-Canonical Structure EF_external_function: EF Sig_signature :=
-  mkEF Sig_signature
-       external_function_eq
-       (fun ef => match ef with EF_external _ _ => true | _ => false end)
-       ef_sig.
-
-Canonical Structure Fundef_C: Fundef F_C EF_external_function_ext :=
-  mkFundef F_C EF_external_function_ext
-           (fun fd =>
-              match fd with
-                | Csyntax.Internal f => inl f
-                | Csyntax.External ef targs tres cc => inr (ef, targs, tres, cc)
-              end).
-Canonical Structure Fundef_Clight: Fundef F_Clight EF_external_function_ext :=
-  mkFundef F_Clight EF_external_function_ext
-           (fun fd =>
-              match fd with
-                | Clight.Internal f => inl f
-                | Clight.External ef targs tres cc => inr (ef, targs, tres, cc)
-              end).
-Canonical Structure Fundef_common (fT:F Sig_signature): Fundef fT EF_external_function :=
-  mkFundef fT EF_external_function
-           (fun fd =>
-              match fd with
-                | AST.Internal f => inl f
-                | AST.External ef => inr ef
-              end).
-
-Canonical Structure V_type: V := mkV Ctypes.type_eq.
-Canonical Structure V_unit: V := mkV unit_eq.
-
-Canonical Structure Language_C: Language := mkLanguage Fundef_C V_type.
-Canonical Structure Language_Clight: Language := mkLanguage Fundef_Clight V_type.
-Canonical Structure Language_Csharpminor: Language := mkLanguage (Fundef_common F_Csharpminor) V_unit.
-Canonical Structure Language_Cminor: Language := mkLanguage (Fundef_common F_Cminor) V_unit.
-Canonical Structure Language_CminorSel: Language := mkLanguage (Fundef_common F_CminorSel) V_unit.
-Canonical Structure Language_RTL: Language := mkLanguage (Fundef_common F_RTL) V_unit.
-Canonical Structure Language_LTL: Language := mkLanguage (Fundef_common F_LTL) V_unit.
-Canonical Structure Language_Linear: Language := mkLanguage (Fundef_common F_Linear) V_unit.
-Canonical Structure Language_Mach: Language := mkLanguage (Fundef_common F_Mach) V_unit.
-Canonical Structure Language_Asm: Language := mkLanguage (Fundef_common F_Asm) V_unit.
 
 (** Linker definition *)
 Section LINKER.
@@ -194,7 +63,7 @@ Inductive globdef_linkable: forall (g1 g2:globdef fundefT vT), Prop :=
 
 (** `linkable` decidabilities. *)
 
-Definition globfun_linkable_dec (f1 f2:fundefT): {globfun_linkable f1 f2} + {~ globfun_linkable f1 f2}.
+Lemma globfun_linkable_dec (f1 f2:fundefT): {globfun_linkable f1 f2} + {~ globfun_linkable f1 f2}.
 Proof.
   destruct (fundef_dec f1) as [i1|e1] eqn:Hf1.
   { right. intro X. inv X.
@@ -210,7 +79,7 @@ Proof.
     + right. contradict n. inv n; clarify.
 Defined.
 
-Definition init_data_dec (v1 v2:init_data): {v1 = v2} + {v1 <> v2}.
+Lemma init_data_dec (v1 v2:init_data): {v1 = v2} + {v1 <> v2}.
 Proof.
   decide equality;
   (try apply Int.eq_dec);
@@ -221,7 +90,7 @@ Proof.
   (try apply ident_eq).
 Defined.
 
-Definition globvar_linkable_dec (v1 v2:globvar vT): {globvar_linkable v1 v2} + {~ globvar_linkable v1 v2}.
+Lemma globvar_linkable_dec (v1 v2:globvar vT): {globvar_linkable v1 v2} + {~ globvar_linkable v1 v2}.
 Proof.
   destruct v1 as [info1 init1 readonly1 volatile1].
   destruct v2 as [info2 init2 readonly2 volatile2].
@@ -243,7 +112,7 @@ Proof.
   { right. contradict n. inv n. auto. }
 Defined.
 
-Definition globdef_linkable_dec (g1 g2:globdef fundefT vT): {globdef_linkable g1 g2} + {~ globdef_linkable g1 g2}.
+Lemma globdef_linkable_dec (g1 g2:globdef fundefT vT): {globdef_linkable g1 g2} + {~ globdef_linkable g1 g2}.
 Proof.
   destruct g1 as [f1|v1], g2 as [f2|v2].
   { destruct (globfun_linkable_dec f1 f2).
