backend/Constpropproof_linker.v
@@ -1,4 +1,5 @@
 Require Import Classical.
+Require Import WFType paco.
 Require Import Coqlib.
 Require Import Maps Maps_linker.
 Require Import AST.
@@ -10,6 +11,8 @@ Require Import Memory.
 Require Import Events.
 Require Import Globalenvs.
 Require Import Smallstep.
+Require Import Language Linker Linkeq.
+Require Import ProgramLSim FunctionLSim.
 Require Import Op.
 Require Import Registers.
 Require Import RTL.
@@ -24,10 +27,7 @@ Require Import ConstpropOp.
 Require Import Constprop.
 Require Import ConstpropOpproof.
 Require Import Constpropproof.
-Require Import LinkerSpecification Linkeq.
-Require Import ProgramLSim.
-Require Import RTLLSim ValueAnalysis_linker.
-Require Import WFType paco.
+Require Import RTL_linker ValueAnalysis_linker.
 
 Set Implicit Arguments.
 
@@ -39,14 +39,14 @@ Hypothesis TRANSF: transf_program prog = tprog.
 Section FUTURE.
 
 Variable (fprog ftprog:program).
-Hypothesis (Hfsim: @program_weak_lsim Language_RTL Language_RTL id (@Errors.OK _) transf_V
+Hypothesis (Hfsim: @program_weak_lsim Language_RTL Language_RTL transf_sigT transf_efT transf_vT
                                       fprog ftprog).
 
 Hypothesis (Hfprog: program_linkeq Language_RTL prog fprog).
 Hypothesis (Hftprog: program_linkeq Language_RTL tprog ftprog).
 
 Let globfun_weak_lsim :=
-  @globfun_lsim Language_RTL Language_RTL id (@Errors.OK _)
+  @globfun_lsim Language_RTL Language_RTL transf_sigT transf_efT
                 (fun _ _ _ _ => True)
                 fprog ftprog.
 
@@ -421,11 +421,11 @@ Proof.
   intros. inv H0. inv H. inv STACKS. inv RES. constructor. 
 Qed.
 
-Inductive match_states_ext n st tst: Prop :=
+Inductive match_states_ext i st tst: Prop :=
 | match_states_ext_intro
-    (Hmatch: match_states n st tst)
     (Hsrc: sound_state_ext fprog st)
     (Htgt: sound_state_ext ftprog tst)
+    (Hmatch: match_states i st tst)
 .
 
 End FUTURE.
@@ -435,11 +435,14 @@ End FUTURE.
 Inductive mrelT_sem (mrel:unit) (fprog ftprog:program) (i:WF.t) (s1 s2:state): Prop :=
 | mrelT_sem_intro n
     (MEASURE: i = WF.from_nat n)
+    (Hsrc: sound_state_ext fprog s1)
+    (Htgt: sound_state_ext ftprog s2)
     (MS: match_states fprog n s1 s2 \/ match_call fprog ftprog n s1 s2)
 .
 
-Definition mrelT_ops: mrelT_opsT unit :=
+Definition mrelT_ops: mrelT_opsT Language_ext_RTL Language_ext_RTL unit :=
   mkmrelT_opsT
+    Language_ext_RTL Language_ext_RTL
     mrelT_sem
     (fun _ v1 v2 => Val.lessdef v1 v2)
     (fun _ _ => True)
@@ -454,7 +457,10 @@ Proof.
   - apply IHv1. auto.
 Qed.
 
-Program Definition mrelT_props: mrelT_propsT mrelT_ops := mkmrelT_propsT _ _ _ _ _ _ _.
+Program Definition mrelT_props:
+  @mrelT_propsT Language_ext_RTL Language_ext_RTL
+                transf_sigT transf_efT transf_vT _ mrelT_ops :=
+  mkmrelT_propsT _ _ _ _ _ _ _.
 Next Obligation. repeat constructor. Qed.
 Next Obligation. repeat constructor. Qed.
 Next Obligation. inv H. auto. Qed.
@@ -462,25 +468,33 @@ Next Obligation.
   exploit transf_initial_states; eauto. intros [n2 [s2' [Hs2' Hinit]]].
   generalize (initial_state_unique Hs2' H2). intro. subst.
   exists tt. eexists. econstructor; eauto.
+  - apply sound_initial. auto.
+  - apply sound_initial. auto.
 Qed.
 Next Obligation.
   apply (mrelT_ops_lessdef_list mrel args1 args2) in Hargs.
   inv Hs0. inv Hmrel. destruct MS as [MS|MS]; inv MS.
+  inv Hfd1. destruct fd2; inv Hfd2.
 
   (* external function *)
   exploit external_call_mem_extends; eauto.
   intros [v' [m2' [A [B [C D]]]]].
-  exists tt. eexists. eexists. eexists. eexists. split; eauto. split.
+  exists tt. eexists. eexists. eexists. eexists. split; eauto.
+  cut (step (Genv.globalenv p2) (Callstate cs2 (External ef2) args2 m2) evt (Returnstate cs2 v' m2')).
+  { intro S. split; eauto. split; auto. econstructor; eauto.
+    - eapply sound_past_step; eauto. econstructor. eauto.
+    - eapply sound_past_step; eauto.
+    - left. econstructor; eauto.
+  }
   eapply exec_function_external; eauto.
   eapply external_call_symbols_preserved; eauto.
   apply symbols_preserved. auto. apply varinfo_preserved. auto.
-  repeat (econstructor; eauto).
 Qed.
 
 Section STATE_LSIM.
   
 Variable (fprog ftprog:program).
-Hypothesis (Hfsim: @program_weak_lsim Language_RTL Language_RTL id (@Errors.OK _) transf_V
+Hypothesis (Hfsim: @program_weak_lsim Language_RTL Language_RTL transf_sigT transf_efT transf_vT
                                       fprog ftprog).
 
 Hypothesis (Hfprog: program_linkeq Language_RTL prog fprog).
@@ -488,7 +502,8 @@ Hypothesis (Hftprog: program_linkeq Language_RTL tprog ftprog).
 
 Lemma match_states_state_lsim es es' eF F i s1 s1'
       (MS: match_states_ext fprog ftprog i s1 s1'):
-  state_lsim mrelT_ops fprog ftprog es es' eF F (WF.from_nat i) s1 s1'.
+  @state_lsim Language_ext_RTL Language_ext_RTL transf_sigT _
+              mrelT_ops fprog ftprog es es' eF F (WF.from_nat i) s1 s1'.
 Proof.
   revert F i s1 s1' MS. pcofix CIH. intros F i s1 s1' MS. pfold.
   inversion MS. destruct (classic (exists r, final_state s1 r)).
@@ -503,6 +518,8 @@ Proof.
   { eexists. exists s2'. exists tt.
     split; [destruct Hmatch2; left; apply plus_one; auto|].
     split; auto. split; [econstructor; eauto|].
+    { eapply sound_past_step; eauto. }
+    { eapply sound_past_step; eauto. }
     destruct Hmatch2 as [Hmatch2|Hmatch2].
     - apply _state_lsim_or_csim_lsim. right. apply CIH.
       constructor; auto.
@@ -511,6 +528,8 @@ Proof.
     - inversion Hmatch2. subst. eapply _state_lsim_or_csim_csim; eauto.
       + apply (mrelT_ops_lessdef_list tt). auto.
       + econstructor; eauto.
+        * eapply sound_past_step; eauto.
+        * eapply sound_past_step; eauto.
       + intros. subst. inversion Hst2_mem. subst. destruct MS0 as [MS0|MS0]; [|inv MS0].
         right. apply CIH. constructor; auto.
   }
@@ -518,6 +537,7 @@ Proof.
     split; [right; split; [subst; econstructor|constructor; eauto]|].
     split; [auto|].
     split; [econstructor; eauto|].
+    { eapply sound_past_step; eauto. }
     destruct Hmatch2 as [Hmatch2|Hmatch2].
     - apply _state_lsim_or_csim_lsim. right. apply CIH.
       constructor; auto.
@@ -525,17 +545,19 @@ Proof.
     - inversion Hmatch2. subst. eapply _state_lsim_or_csim_csim; eauto.
       + apply (mrelT_ops_lessdef_list tt). auto.
       + econstructor; eauto.
+        eapply sound_past_step; eauto.
       + intros. subst. inversion Hst2_mem. subst. destruct MS0 as [MS0|MS0]; [|inv MS0].
         right. apply CIH. constructor; auto.
   }
 Qed.
 
 Lemma transf_function_lsim f:
-  function_lsim mrelT_ops fprog ftprog f (transf_function (romem_for_program prog) f).
+  @function_lsim Language_ext_RTL Language_ext_RTL transf_sigT _
+                 mrelT_ops fprog ftprog f (transf_function (romem_for_program prog) f).
 Proof.
   constructor. intros. pfold. constructor; subst; auto.
   { intros ? Hfinal. inv Hfinal. }
-  intros. inversion Hst2_src. subst.
+  intros. destruct fd_src; inv Hfd_src. destruct fd_tgt; inv Hfd_tgt. inversion Hst2_src. subst.
   inv Hmrel_entry. destruct MS as [MS|MS]; inversion MS; subst.
 
   (* internal function *)
@@ -544,16 +566,32 @@ Proof.
   assert (X: exists bc ae, ematch bc (init_regs args_src (fn_params f)) ae).
   { exploit sound_past_step; eauto. intro X. inv X.
     exploit Hsound. apply program_linkeq_romem_le; eauto. intro X. inv X.
-    eexists. eexists. eauto. }
+    eexists. eexists. eauto.
+  }
   destruct X as (bc1 & ae1 & MATCH).
   simpl. unfold transf_function.
   exists (WF.from_nat O). eexists. exists tt. split.
   left. apply plus_one. constructor; eauto.
   simpl. split; [auto|].
-  cut (match_states fprog O
-                    (State cs_entry_src f (Vptr stk Int.zero) (fn_entrypoint f)
+  assert (Hstep: step (Genv.globalenv ftprog)
+                      (Callstate es_tgt
+                                 (Internal (transf_function (romem_for_program prog) f)) args_tgt
+                                 mem_entry_tgt) E0
+                      (State es_tgt
+                             {|
+                               fn_sig := fn_sig f;
+                               fn_params := fn_params f;
+                               fn_stacksize := fn_stacksize f;
+                               fn_code := PTree.map
+                                            (transf_instr f (analyze (romem_for_program prog) f)
+                                                          (romem_for_program prog)) (fn_code f);
+                               fn_entrypoint := fn_entrypoint f |} (Vptr stk Int.zero)
+                             (fn_entrypoint f) (init_regs args_tgt (fn_params f)) m2')).
+  { apply (exec_function_internal _ es_tgt (transf_function (romem_for_program prog) f)). eauto. }
+  cut (match_states fprog 0
+                    (State es_src f (Vptr stk Int.zero) (fn_entrypoint f)
                            (init_regs args_src (fn_params f)) m')
-                    (State cs_entry_tgt
+                    (State es_tgt
                            {|
                              fn_sig := fn_sig f;
                              fn_params := fn_params f;
@@ -564,12 +602,13 @@ Proof.
                              fn_entrypoint := fn_entrypoint f |} (Vptr stk Int.zero)
                            (fn_entrypoint f) (init_regs args_tgt (fn_params f)) m2')).
   { intro MS2. split; [econstructor; eauto|].
+    { eapply sound_past_step; eauto. }
+    { eapply sound_past_step; eauto. }
     constructor. left. apply match_states_state_lsim. constructor; auto.
     - eapply sound_past_step; eauto.
     - eapply sound_past_step; eauto.
-      apply (exec_function_internal _ cs_entry_tgt (transf_function (romem_for_program prog) f)). auto.
   }
-  simpl. econstructor; eauto.
+  econstructor; eauto.
   constructor.
   apply init_regs_lessdef; auto.
   apply program_linkeq_romem_le. auto.
@@ -578,8 +617,8 @@ Qed.
 End STATE_LSIM.
 
 Lemma Constprop_program_lsim:
-  @program_lsim Language_RTL Language_RTL id (@Errors.OK _) transf_V
-                (function_lsim mrelT_ops)
+  @program_lsim Language_RTL Language_RTL transf_sigT transf_efT transf_vT
+                (@function_lsim Language_ext_RTL Language_ext_RTL transf_sigT _ mrelT_ops)
                 prog tprog.
 Proof.
   generalize transf_function_lsim.
