backend/RTL_linker.v
@@ -1,0 +1,172 @@
+Require Import RelationClasses.
+Require Import Coqlib.
+Require Import paco.
+Require Import WFType.
+Require Import Maps.
+Require Import AST.
+Require Import Integers.
+Require Import Values.
+Require Import Events.
+Require Import Memory.
+Require Import Globalenvs.
+Require Import Smallstep.
+Require Import Op.
+Require Import Registers.
+Require Import Language Linker ProgramLSim.
+Require Import RTL.
+
+Set Implicit Arguments.
+
+(* common definitions/lemmas on RTL *)
+
+Definition transf_sigT := fun (sig:signature) => sig.
+Definition transf_efT := fun (ef:external_function) => Errors.OK ef.
+Definition transf_vT := fun (tt:unit) => Errors.OK tt.
+Lemma transf_efT_sigT:
+  forall (ef_src : efT Language_RTL) (ef_tgt : efT Language_RTL),
+    Errors.OK ef_src = Errors.OK ef_tgt ->
+    id (EF_sig (efT Language_RTL) ef_src) =
+    EF_sig (efT Language_RTL) ef_tgt.
+Proof. intros. inv H. auto. Qed.
+
+Lemma initial_state_unique p s1 s2
+      (H1: initial_state p s1)
+      (H2: initial_state p s2):
+  s1 = s2.
+Proof.
+  inv H1. inv H2. unfold ge, ge0 in *.
+  rewrite H in H1. inv H1. rewrite H0 in H5. inv H5. rewrite H3 in H6. inv H6.
+  auto.
+Qed.
+
+Lemma Fundef_funsig f: Fundef_sig (Fundef_common F_RTL) f = RTL.funsig f.
+Proof. unfold Fundef_sig, Fundef_dec. simpl. destruct f; auto. Qed.
+
+Lemma initial_state_equiv p s:
+  Language.initial_state Language_ext_RTL p s <-> RTL.initial_state p s.
+Proof.
+  constructor; intro X; inv X; simpl in *; econstructor; eauto.
+  - rewrite <- Fundef_funsig. auto.
+  - rewrite Fundef_funsig. auto.
+Qed.
+
+Lemma final_state_equiv p r:
+  Language.final_state Language_ext_RTL p r <-> RTL.final_state p r.
+Proof.
+  constructor; intro X; inv X; simpl in *; econstructor; eauto.
+Qed.
+
+Section FUTURE.
+
+Variable (fprog ftprog:program).
+Hypothesis (Hfsim: @program_weak_lsim Language_RTL Language_RTL transf_sigT transf_efT transf_vT
+                                      fprog ftprog).
+
+Let globfun_weak_lsim :=
+  @globfun_lsim Language_RTL Language_RTL id (@Errors.OK _)
+                (fun _ _ _ _ => True)
+                fprog ftprog.
+
+Let ge := Genv.globalenv fprog.
+Let tge := Genv.globalenv ftprog.
+
+Lemma symbols_preserved:
+  forall (s: ident), Genv.find_symbol tge s = Genv.find_symbol ge s.
+Proof (symbols_preserved transf_efT_sigT Hfsim).
+
+Lemma varinfo_preserved:
+  forall b, Genv.find_var_info tge b = Genv.find_var_info ge b.
+Proof.
+  intros. exploit varinfo_preserved; try exact transf_efT_sigT; try exact Hfsim.
+  instantiate (1 := b). unfold ge, tge, fundef. simpl in *.
+  match goal with
+    | [|- context[match ?v1 with | Some _ => match ?v2 with | Some _ => _ | None => _ end | None => _ end]] =>
+      destruct v1, v2; intros; auto; inv H
+  end.
+  destruct g0; auto.
+Qed.
+
+Lemma funct_ptr_translated:
+  forall (b: block) (f: RTL.fundef),
+  Genv.find_funct_ptr ge b = Some f ->
+  exists tf, Genv.find_funct_ptr tge b = Some tf /\
+             fundef_weak_lsim Language_RTL Language_RTL id ge tge f tf.
+Proof (funct_ptr_translated transf_efT_sigT Hfsim).
+
+Lemma functions_translated:
+  forall (v: val) (f: RTL.fundef),
+  Genv.find_funct ge v = Some f ->
+  exists tf, Genv.find_funct tge v = Some tf /\
+             fundef_weak_lsim Language_RTL Language_RTL id ge tge f tf.
+Proof (functions_translated transf_efT_sigT Hfsim).
+
+Lemma find_function_translated_Renumber:
+  forall ros rs fd,
+  find_function ge ros rs = Some fd ->
+  exists tfd, find_function tge ros rs = Some tfd /\
+              fundef_weak_lsim Language_RTL Language_RTL id ge tge fd tfd.
+Proof.
+  unfold find_function; intros; destruct ros.
+- apply functions_translated; auto.
+- rewrite symbols_preserved. destruct (Genv.find_symbol ge i).
+  apply funct_ptr_translated; auto.
+  discriminate.
+Qed.
+
+Lemma find_function_translated_CSE:
+  forall ros rs fd rs',
+  find_function ge ros rs = Some fd ->
+  CSEproof.regs_lessdef rs rs' ->
+  exists tfd, find_function tge ros rs' = Some tfd /\
+              fundef_weak_lsim Language_RTL Language_RTL id ge tge fd tfd.
+Proof.
+  unfold find_function; intros; destruct ros.
+- specialize (H0 r). inv H0.
+  apply functions_translated; auto.
+  rewrite <- H2 in H; discriminate.
+- rewrite symbols_preserved. destruct (Genv.find_symbol ge i).
+  apply funct_ptr_translated; auto.
+  discriminate.
+Qed.
+
+Lemma find_function_translated_Tailcall:
+  forall ros rs fd rs',
+  find_function ge ros rs = Some fd ->
+  Tailcallproof.regset_lessdef rs rs' ->
+  exists tfd, find_function tge ros rs' = Some tfd /\
+              fundef_weak_lsim Language_RTL Language_RTL id ge tge fd tfd.
+Proof.
+  unfold find_function; intros; destruct ros.
+- specialize (H0 r). inv H0.
+  apply functions_translated; auto.
+  rewrite <- H2 in H; discriminate.
+- rewrite symbols_preserved. destruct (Genv.find_symbol ge i).
+  apply funct_ptr_translated; auto.
+  discriminate.
+Qed.
+
+Lemma find_function_translated_Constprop:
+  forall ros rs fd rs',
+  find_function ge ros rs = Some fd ->
+  Constpropproof.regs_lessdef rs rs' ->
+  exists tfd, find_function tge ros rs' = Some tfd /\
+              fundef_weak_lsim Language_RTL Language_RTL id ge tge fd tfd.
+Proof.
+  unfold find_function; intros; destruct ros.
+- specialize (H0 r). inv H0.
+  apply functions_translated; auto.
+  rewrite <- H2 in H; discriminate.
+- rewrite symbols_preserved. destruct (Genv.find_symbol ge i).
+  apply funct_ptr_translated; auto.
+  discriminate.
+Qed.
+
+Lemma sig_preserved:
+  forall f tf,
+    fundef_weak_lsim Language_RTL Language_RTL id ge tge f tf ->
+    funsig tf = funsig f.
+Proof.
+  intros. inv H. inv Hsig. rewrite ? Fundef_funsig in Hsig0. auto.
+Qed.
+
+End FUTURE.
