common/Adequacy.v
@@ -1,0 +1,223 @@
+Require Import Coqlib Coqlib_linker.
+Require Import paco.
+Require Import WFType.
+Require Import Maps.
+Require Import AST.
+Require Import Integers.
+Require Import Values.
+Require Import Events.
+Require Import Memory.
+Require Import Globalenvs.
+Require Import Smallstep.
+Require Import Language Linker.
+Require Import ProgramLSim FunctionLSim.
+
+Set Implicit Arguments.
+
+Section ADEQUACY.
+
+Variable (lang_src lang_tgt:Language_ext).
+
+Let sigT_src := lang_src.(sigT).
+Let fT_src := lang_src.(fT).
+Let efT_src := lang_src.(efT).
+Let fundefT_src := lang_src.(fundefT).
+Let vT_src := lang_src.(vT).
+
+Let f_sig_src := fT_src.(F_sig).
+Let ef_sig_src := efT_src.(EF_sig).
+Let fd_sig_src := fundefT_src.(Fundef_sig).
+Let ef_dec_src := efT_src.(EF_dec).
+Let fundef_dec_src := fundefT_src.(Fundef_dec).
+Let v_dec_src := vT_src.(V_dec).
+
+Let sigT_tgt := lang_tgt.(sigT).
+Let fT_tgt := lang_tgt.(fT).
+Let efT_tgt := lang_tgt.(efT).
+Let fundefT_tgt := lang_tgt.(fundefT).
+Let vT_tgt := lang_tgt.(vT).
+
+Let f_sig_tgt := fT_tgt.(F_sig).
+Let ef_sig_tgt := efT_tgt.(EF_sig).
+Let fd_sig_tgt := fundefT_tgt.(Fundef_sig).
+Let ef_dec_tgt := efT_tgt.(EF_dec).
+Let fundef_dec_tgt := fundefT_tgt.(Fundef_dec).
+Let v_dec_tgt := vT_tgt.(V_dec).
+
+Variable (transf_sigT: forall (ef:sigT_src), sigT_tgt).
+Variable (transf_efT: forall (ef:efT_src), Errors.res efT_tgt).
+Variable (transf_vT: forall (v:vT_src), Errors.res vT_tgt).
+Hypothesis transf_efT_sigT: forall ef_src ef_tgt (H: transf_efT ef_src = Errors.OK ef_tgt), transf_sigT (ef_sig_src ef_src) = ef_sig_tgt ef_tgt.
+Hypothesis transf_sigT_main: transf_sigT lang_src.(signature_main) = lang_tgt.(signature_main).
+
+Variable (mrelT:Type).
+Variable (mrelT_ops:mrelT_opsT lang_src lang_tgt mrelT).
+Hypothesis (mrelT_props:mrelT_propsT transf_sigT transf_efT transf_vT mrelT_ops).
+
+Variable (prog_src:lang_src.(progT)).
+Variable (prog_tgt:lang_tgt.(progT)).
+Hypothesis
+  (Hsim: @program_lsim lang_src lang_tgt transf_sigT transf_efT transf_vT
+                       (function_lsim transf_sigT mrelT_ops)
+                       prog_src prog_tgt).
+
+Lemma Hweak_sim:
+  @program_weak_lsim lang_src lang_tgt transf_sigT transf_efT transf_vT
+                     prog_src prog_tgt.
+Proof. eapply program_lsim_aux_le; eauto. Qed.
+Hint Resolve Hweak_sim.
+
+Inductive match_stackframes: forall (height:nat) (mrel:mrelT) (es_src:lang_src.(contT)) (es_tgt:lang_tgt.(contT)), Prop :=
+| match_stackframes_nil mrel_init:
+    match_stackframes 0 mrel_init lang_src.(empty_cont) lang_tgt.(empty_cont)
+| match_stackframes_cons
+    height ps_src ps_tgt es_src es_tgt
+    emrel mrel
+    (Hp: match_stackframes height emrel ps_src ps_tgt)
+    (Hmrel_le: mrelT_ops.(le) emrel mrel)
+    (Hreturn:
+       forall rmrel ri st_src st_tgt mem_src mem_tgt vres_src vres_tgt
+              (Hvres: mrelT_ops.(sem_value) rmrel vres_src vres_tgt)
+              (Hst_src: st_src = lang_src.(mkReturnstate) es_src vres_src mem_src)
+              (Hst_tgt: st_tgt = lang_tgt.(mkReturnstate) es_tgt vres_tgt mem_tgt)
+              (Hrmrel_le: mrelT_ops.(le_public) mrel rmrel)
+              (Hst_mem: mrelT_ops.(sem) rmrel prog_src prog_tgt ri st_src st_tgt),
+         state_lsim transf_sigT mrelT_ops prog_src prog_tgt ps_src ps_tgt emrel rmrel ri st_src st_tgt):
+    match_stackframes (S height) mrel es_src es_tgt
+.
+
+Inductive match_states (i:WF.t) (st_src:lang_src.(stateT)) (st_tgt:lang_tgt.(stateT)): Prop :=
+| match_states_intro
+    height es_src es_tgt
+    emrel mrel
+    (Hp: match_stackframes height emrel es_src es_tgt)
+    (Hmrel_le: mrelT_ops.(le) emrel mrel)
+    (Hsim: state_lsim transf_sigT mrelT_ops prog_src prog_tgt es_src es_tgt emrel mrel i st_src st_tgt)
+.
+
+Lemma program_sim_forward_simulation:
+  forward_simulation (lang_src.(semantics) prog_src) (lang_tgt.(semantics) prog_tgt).
+Proof.
+  eapply (Forward_simulation
+            (lang_src.(semantics) prog_src) (lang_tgt.(semantics) prog_tgt)
+            WF.wf match_states).
+  { (* initial *)
+    intros. destruct H as [b [f [m0 [Hm0 [Hb [Hf [Hsig ?]]]]]]]. subst.
+    exploit funct_ptr_translated; eauto. intros [tf [A B]].
+    assert (Hinitial_tgt: initial_state lang_tgt prog_tgt (lang_tgt.(mkCallstate) lang_tgt.(empty_cont) tf nil m0)).
+    { exists b. exists tf. exists m0.
+      split. eapply program_lsim_init_mem_match; eauto.
+      split. replace (prog_main prog_tgt) with (prog_main prog_src).
+        erewrite symbols_preserved; eauto. auto.
+        destruct Hsim as [_ Hmain]. auto.
+      repeat (split; auto).
+      rewrite <- transf_sigT_main, <- Hsig. inv B. inv Hsig0. auto.
+    }
+    exploit (mrelT_props.(Hmrel_i_init)); eauto.
+    { eexists. eexists. eexists. eauto. }
+    intros [mrel_init [i_init Hinitial]].
+    exists i_init. exists (lang_tgt.(mkCallstate) lang_tgt.(empty_cont) tf nil m0). split; auto.
+    econstructor.
+    { apply match_stackframes_nil. }
+    { destruct mrelT_props. reflexivity. }
+    exploit funct_ptr_translated'; try exact transf_efT_sigT; eauto.
+    intros [tf' [Htf' Hfundef_sim]]. rewrite A in Htf'. symmetry in Htf'. inv Htf'.
+    inv Hfundef_sim.
+    destruct (Fundef_dec (fundefT lang_src) f) as [f_src|ef_src] eqn:Hfundef_src,
+             (Fundef_dec (fundefT lang_tgt) tf) as [f_tgt|ef_tgt] eqn:Hfundef_tgt;
+    try (inv Hsim0; fail).
+    - exploit Hsim0; try reflexivity. unfold F_future_lsim. intros.
+      destruct H as [Hfunction_sim Hfunction_sig].
+      exploit Hfunction_sim; eauto.
+      intro X. inv X. eapply Hlsim; eauto. constructor.
+    - inv Hsim0. pfold. constructor.
+      { intros r Hr. inv Hr. exploit Hfinal_not_call; eauto. }
+      intros. exploit (mrelT_props.(Hexternal_call)); eauto.
+      { constructor. }
+      intros [res [m2 [s2' [res' [m2' [mrel2 [i2 [? [? [Hst2_tgt [Hmrel2 [Hmrel2_val Hmrel2_le]]]]]]]]]]]].
+      exists i2. exists s2'. exists mrel2.
+      split; [left; apply plus_one; auto|].
+      split; [apply mrelT_props.(le_public_le); auto|].
+      split; auto. subst. econstructor. left.
+      pfold. eapply _state_lsim_return; eauto.
+  }
+ { (* final *)
+    simpl. intros. inv H0. inv H. punfold Hsim0. inv Hsim0.
+    - inv Hst_src. apply HmkReturnstate_inj in H. destruct H as [? [? ?]]. subst.
+      inv H0. auto.
+    - apply HmkReturnstate_inj in Hst_src. destruct Hst_src as [? [? ?]]. subst.
+      revert height emrel Hmrel_le Hmrel_le_public Hp.
+      refine (strong_nat_ind _ _). intros height IHheight emrel Hmrel_le Hmrel_le_public Hp.
+      inversion Hp; symmetry in H0; subst.
+      { exploit (mrelT_props.(sem_value_int)); eauto. intro. subst.
+        econstructor. eauto.
+      }
+      { exploit Hreturn; eauto. intro Hsim'.
+        punfold Hsim'. inv Hsim'.
+        { inv Hst_src. apply HmkReturnstate_inj in H. destruct H as [? [? ?]]. subst.
+          inv Hst_tgt. apply HmkReturnstate_inj in H1. destruct H1 as [? [? ?]]. subst.
+          inv H0. econstructor. eauto.
+        }
+        { apply HmkReturnstate_inj in Hst_src. destruct Hst_src as [? [? ?]]. subst.
+          apply HmkReturnstate_inj in Hst_tgt. destruct Hst_tgt as [? [? ?]]. subst.
+          assert (Hle: mrelT_ops.(le) emrel0 mrel).
+          { destruct mrelT_props. etransitivity; eauto. }
+          eauto.
+        }
+        { exfalso. eapply Hnfinal. econstructor. eauto. }
+      }
+    - exfalso. eapply Hnfinal. econstructor. eauto.
+  }
+  { (* progress & preservation *)
+    intros. inv H0.
+    revert height i s2 es_src es_tgt emrel mrel Hp Hmrel_le Hsim0.
+    refine (strong_nat_ind _ _). intros height IHheight. intros.
+    punfold Hsim0. inv Hsim0.
+    - (* term *)
+      inv Hst_src. exfalso. eapply Hfinal_not_progress.
+      eexists. eexists. eexists. apply H.
+    - (* return *)
+      inversion Hp; subst.
+      { exfalso. eapply Hfinal_not_progress.
+        eexists. eexists. eexists. apply H.
+      }
+      assert (Hmrel_le': mrelT_ops.(le) emrel0 mrel).
+      { destruct mrelT_props. etransitivity; eauto. }
+      exploit Hreturn; eauto.
+    - (* step *)
+      exploit Hpreserve; eauto. intros [i2 [st2_tgt [mrel2 [Hstep2 [Hle2 [Hmrel2 Hsim2]]]]]].
+      assert (Hmrel2_le: mrelT_ops.(le) emrel mrel2).
+      { destruct mrelT_props. etransitivity; eauto. }
+      exists i2. exists st2_tgt. split; auto.
+      inv Hsim2.
+      { pclearbot. econstructor; eauto. }
+      econstructor.
+      { eapply match_stackframes_cons; eauto.
+        instantiate (1 := cont_tgt). instantiate (1 := cont_src). intros. subst.
+        exploit Hreturn; eauto. intro Hsim2. pclearbot. eauto.
+      }
+      { destruct mrelT_props. reflexivity. }
+      inv Hfundef. exploit funct_ptr_translated'; try exact transf_efT_sigT; eauto.
+      intros [tf [Htf Hfundef_sim]]. unfold Genv.find_funct_ptr in Htf. rewrite Htgt in Htf. symmetry in Htf. inv Htf.
+      inv Hfundef_sim.
+      destruct (Fundef_dec (fundefT lang_src) fundef_src) as [f_src|ef_src] eqn:Hfundef_src,
+               (Fundef_dec (fundefT lang_tgt) fundef_tgt) as [f_tgt|ef_tgt] eqn:Hfundef_tgt;
+      try (inv Hsim0; fail).
+      + exploit Hsim0; try reflexivity. unfold F_future_lsim. intros.
+        destruct H0 as [Hfunction_sim Hfunction_sig].
+        exploit Hfunction_sim; eauto.
+        intro X. inv X. eapply Hlsim; eauto.
+      + inv Hsim0. pfold. constructor.
+        { intros ? Hfinal. inv Hfinal. exploit Hfinal_not_call; eauto. }
+        intros. exploit (mrelT_props.(Hexternal_call)); eauto.
+        intros [res [m3 [s3' [res' [m3' [mrel3 [i3 [? [? [Hst3_tgt [Hmrel3 [Hmrel3_val Hmrel3_le]]]]]]]]]]]].
+        exists i3. exists s3'. exists mrel3.
+        split; [left; apply plus_one; auto|].
+        split; [apply mrelT_props.(le_public_le); auto|].
+        split; auto. subst. econstructor. left.
+        pfold. eapply _state_lsim_return; eauto.
+  }
+  { eapply symbols_preserved; eauto. }
+Qed.
+
+End ADEQUACY.
