common/FunctionLSim.v
@@ -1,0 +1,204 @@
+Require Import RelationClasses.
+Require Import Coqlib.
+Require Import paco.
+Require Import WFType.
+Require Import Maps.
+Require Import AST.
+Require Import Integers.
+Require Import Values.
+Require Import Events.
+Require Import Memory.
+Require Import Globalenvs.
+Require Import Smallstep.
+Require Import Language Linker.
+Require Import ProgramLSim.
+
+Set Implicit Arguments.
+
+Section LSIM.
+
+Variable (lang_src lang_tgt:Language_ext).
+
+Let sigT_src := lang_src.(sigT).
+Let fT_src := lang_src.(fT).
+Let efT_src := lang_src.(efT).
+Let fundefT_src := lang_src.(fundefT).
+Let vT_src := lang_src.(vT).
+
+Let f_sig_src := fT_src.(F_sig).
+Let ef_sig_src := efT_src.(EF_sig).
+Let fd_sig_src := fundefT_src.(Fundef_sig).
+Let ef_dec_src := efT_src.(EF_dec).
+Let fundef_dec_src := fundefT_src.(Fundef_dec).
+Let v_dec_src := vT_src.(V_dec).
+
+Let sigT_tgt := lang_tgt.(sigT).
+Let fT_tgt := lang_tgt.(fT).
+Let efT_tgt := lang_tgt.(efT).
+Let fundefT_tgt := lang_tgt.(fundefT).
+Let vT_tgt := lang_tgt.(vT).
+
+Let f_sig_tgt := fT_tgt.(F_sig).
+Let ef_sig_tgt := efT_tgt.(EF_sig).
+Let fd_sig_tgt := fundefT_tgt.(Fundef_sig).
+Let ef_dec_tgt := efT_tgt.(EF_dec).
+Let fundef_dec_tgt := fundefT_tgt.(Fundef_dec).
+Let v_dec_tgt := vT_tgt.(V_dec).
+
+Variable (transf_sigT: forall (ef:sigT_src), sigT_tgt).
+Variable (transf_efT: forall (ef:efT_src), Errors.res efT_tgt).
+Variable (transf_vT: forall (v:vT_src), Errors.res vT_tgt).
+Hypothesis transf_efT_sigT: forall ef_src ef_tgt (H: transf_efT ef_src = Errors.OK ef_tgt), transf_sigT (ef_sig_src ef_src) = ef_sig_tgt ef_tgt.
+
+Record mrelT_opsT (t:Type): Type := mkmrelT_opsT {
+  sem :> t -> forall (p_src:lang_src.(progT)) (p_tgt:lang_tgt.(progT)) (i:WF.t) (s1:lang_src.(stateT)) (s2:lang_tgt.(stateT)), Prop;
+  sem_value :> t -> forall (v1 v2:val), Prop;
+  le: t -> t -> Prop;
+  le_public: t -> t -> Prop
+}.
+
+Record mrelT_propsT (t:Type) (ops:mrelT_opsT t): Prop := mkmrelT_propsT {
+  le_preorder: PreOrder ops.(le);
+  le_public_preorder: PreOrder ops.(le_public);
+  le_public_le:
+    forall mrel1 mrel2 (Hle_public: ops.(le_public) mrel1 mrel2),
+      ops.(le) mrel1 mrel2;
+  sem_value_int:
+    forall mrel i v (H: ops.(sem_value) mrel (Vint i) v),
+      v = Vint i;
+  Hmrel_i_init:
+    forall p1 p2 s1 s2
+           (Hp: @program_weak_lsim lang_src lang_tgt transf_sigT transf_efT transf_vT
+                                   p1 p2)
+           (H1: lang_src.(initial_state) p1 s1)
+           (H2: lang_tgt.(initial_state) p2 s2),
+    exists mrel_init i_init,
+      ops.(sem) mrel_init p1 p2 i_init s1 s2;
+  Hexternal_call:
+    forall p1 p2 s1 s2 es1 es2 fd1 fd2 ef1 ef2 args1 args2 m1 m2 evt s1' mrel i
+           (Hp: @program_weak_lsim lang_src lang_tgt transf_sigT transf_efT transf_vT
+                                   p1 p2)
+           (Hs1: s1 = lang_src.(mkCallstate) es1 fd1 args1 m1)
+           (Hs2: s2 = lang_tgt.(mkCallstate) es2 fd2 args2 m2)
+           (Hfd1: fundef_dec_src fd1 = inr ef1)
+           (Hfd2: fundef_dec_tgt fd2 = inr ef2)
+           (Hef: transf_efT ef1 = Errors.OK ef2)
+           (Hmrel: ops.(sem) mrel p1 p2 i s1 s2)
+           (Hs2: lang_src.(step) (Genv.globalenv p1) s1 evt s1')
+           (Hargs: list_forall2 (ops.(sem_value) mrel) args1 args2),
+    exists res1 m1' s2' res2 m2' mrel' i',
+      s1' = lang_src.(mkReturnstate) es1 res1 m1' /\
+      s2' = lang_tgt.(mkReturnstate) es2 res2 m2' /\
+      lang_tgt.(step) (Genv.globalenv p2) s2 evt s2' /\
+      ops.(sem) mrel' p1 p2 i' s1' s2' /\
+      ops.(sem_value) mrel' res1 res2 /\
+      ops.(le_public) mrel mrel'
+}.
+
+Variable (mrelT:Type).
+Variable (mrelT_ops:mrelT_opsT mrelT).
+
+Variable (fprog_src:lang_src.(progT)).
+Variable (fprog_tgt:lang_tgt.(progT)).
+
+Let ge_src := Genv.globalenv fprog_src.
+Let ge_tgt := Genv.globalenv fprog_tgt.
+
+Section STATE_LSIM.
+
+Variable (es_src:lang_src.(contT)).
+Variable (es_tgt:lang_tgt.(contT)).
+Variable (mrel_entry:mrelT).
+
+Inductive _state_lsim_or_csim
+          (state_lsim: mrelT -> WF.t -> lang_src.(stateT) -> lang_tgt.(stateT) -> Prop)
+          (mrel:mrelT) (i:WF.t) (st_src:lang_src.(stateT)) (st_tgt:lang_tgt.(stateT)): Prop :=
+| _state_lsim_or_csim_lsim
+    (Hlsim: state_lsim mrel i st_src st_tgt)
+| _state_lsim_or_csim_csim
+    cont_src fundef_src args_src mem_src
+    (Hst_src: st_src = lang_src.(mkCallstate) cont_src fundef_src args_src mem_src)
+    cont_tgt fundef_tgt args_tgt mem_tgt
+    (Hst_tgt: st_tgt = lang_tgt.(mkCallstate) cont_tgt fundef_tgt args_tgt mem_tgt)
+    (Hfundef: fundef_weak_lsim lang_src lang_tgt transf_sigT ge_src ge_tgt fundef_src fundef_tgt)
+    (Hargs: list_forall2 (mrelT_ops.(sem_value) mrel) args_src args_tgt)
+    (Hmrel: mrelT_ops.(sem) mrel fprog_src fprog_tgt i st_src st_tgt)
+    (Hreturn:
+       forall mrel2 i2 st2_src st2_tgt mem2_src mem2_tgt vres_src vres_tgt
+              (Hvres: mrelT_ops.(sem_value) mrel2 vres_src vres_tgt)
+              (Hst2_src: st2_src = lang_src.(mkReturnstate) cont_src vres_src mem2_src)
+              (Hst2_tgt: st2_tgt = lang_tgt.(mkReturnstate) cont_tgt vres_tgt mem2_tgt)
+              (Hmrel2_le: mrelT_ops.(le_public) mrel mrel2)
+              (Hst2_mem: mrelT_ops.(sem) mrel2 fprog_src fprog_tgt i2 st2_src st2_tgt),
+         state_lsim mrel2 i2 st2_src st2_tgt)
+.
+
+Inductive _state_lsim
+          (state_lsim: mrelT -> WF.t -> lang_src.(stateT) -> lang_tgt.(stateT) -> Prop)
+          (mrel:mrelT) (i:WF.t) (st_src:lang_src.(stateT)) (st_tgt:lang_tgt.(stateT)): Prop :=
+| _state_lsim_term
+    rval
+    (Hst_src: lang_src.(final_state) st_src rval)
+    (Hst_tgt: lang_tgt.(final_state) st_tgt rval)
+
+| _state_lsim_return
+    val_src mem_src (Hst_src: st_src = lang_src.(mkReturnstate) es_src val_src mem_src)
+    val_tgt mem_tgt (Hst_tgt: st_tgt = lang_tgt.(mkReturnstate) es_tgt val_tgt mem_tgt)
+    (Hval: mrelT_ops.(sem_value) mrel val_src val_tgt)
+    (Hmem: mrelT_ops.(sem) mrel fprog_src fprog_tgt i st_src st_tgt)
+    (Hmrel_le_public: mrelT_ops.(le_public) mrel_entry mrel)
+
+| _state_lsim_step
+    (Hnfinal: forall r, ~ lang_src.(final_state) st_src r)
+    (Hpreserve:
+       forall evt st2_src (Hst2_src: lang_src.(step) ge_src st_src evt st2_src),
+         exists i2 st2_tgt (mrel2:mrelT),
+           (plus lang_tgt.(step) ge_tgt st_tgt evt st2_tgt \/
+            star lang_tgt.(step) ge_tgt st_tgt evt st2_tgt /\ WF.rel i2 i) /\
+           mrelT_ops.(le) mrel mrel2 /\
+           mrelT_ops.(sem) mrel2 fprog_src fprog_tgt i2 st2_src st2_tgt /\
+           _state_lsim_or_csim state_lsim mrel2 i2 st2_src st2_tgt)
+.
+Hint Constructors _state_lsim.
+
+Lemma state_lsim_mon: monotone4 _state_lsim.
+Proof.
+  repeat intro; destruct IN; eauto.
+  - eapply _state_lsim_step; eauto.
+    intros. exploit Hpreserve; eauto. intros [i2 [st2_tgt [mrel2 [Hstep [Hle [Hmrel Hsim]]]]]].
+    eexists. eexists. eexists. repeat (split; eauto).
+    inv Hsim.
+    + apply _state_lsim_or_csim_lsim. eauto.
+    + eapply _state_lsim_or_csim_csim; eauto.
+Qed.
+
+Definition state_lsim: _ -> _ -> _ -> _ -> Prop :=
+  paco4 _state_lsim bot4.
+
+End STATE_LSIM.
+
+Inductive function_lsim (func_src:lang_src.(fT)) (func_tgt:lang_tgt.(fT)): Prop :=
+| function_lsim_intro
+    (Hlsim:
+       forall
+         mrel_entry mem_entry_src mem_entry_tgt
+         es_src es_tgt
+         fd_src fd_tgt
+         args_src args_tgt
+         st_src st_tgt
+         i
+         (Hmrel_entry: mrelT_ops.(sem) mrel_entry fprog_src fprog_tgt i st_src st_tgt)
+         (Hfd_src: fundef_dec_src fd_src = inl func_src)
+         (Hfd_tgt: fundef_dec_tgt fd_tgt = inl func_tgt)
+         (Hargs: list_forall2 (mrelT_ops.(sem_value) mrel_entry) args_src args_tgt)
+         (Hst_src: st_src = lang_src.(mkCallstate) es_src fd_src args_src mem_entry_src)
+         (Hst_tgt: st_tgt = lang_tgt.(mkCallstate) es_tgt fd_tgt args_tgt mem_entry_tgt),
+         state_lsim
+           es_src es_tgt mrel_entry
+           mrel_entry i
+           st_src st_tgt)
+.
+
+End LSIM.
+Hint Constructors _state_lsim.
+Hint Resolve state_lsim_mon: paco.
