common/Language.v
@@ -1,0 +1,245 @@
+Require Import RelationClasses.
+Require String.
+Require Import Coqlib Coqlib_linker.
+Require Import Maps Maps_linker.
+Require Import Integers Floats Values AST Globalenvs.
+Require Import Errors Behaviors Compiler Smallstep.
+Require Import Memory.
+
+Set Implicit Arguments.
+
+Definition external_function_ext :=
+  (external_function * Ctypes.typelist * Ctypes.type * calling_convention)%type.
+
+Definition external_function_ext_eq (ef1 ef2: external_function_ext): {ef1 = ef2} + {ef1 <> ef2}.
+Proof.
+  destruct ef1 as [[[ef1 args1] res1] cc1].
+  destruct ef2 as [[[ef2 args2] res2] cc2].
+  decide equality.
+  { destruct b, c.
+    destruct (bool_dec cc_vararg cc_vararg0); [subst|].
+    { destruct (bool_dec cc_structret cc_structret0); [subst|].
+      { left. auto. }
+      { right. contradict n. inv n. auto. }
+    }
+    { right. contradict n. inv n. auto. }
+  }
+  decide equality.
+  { apply Ctypes.type_eq. }
+  decide equality.
+  { apply Ctypes.typelist_eq. }
+  { apply external_function_eq. }
+Defined.
+
+(** Structures *)
+
+Structure Sig: Type := mkSig {
+  Sig_carrier :> Type;
+  Sig_dec: forall (sig1 sig2:Sig_carrier), {sig1 = sig2} + {sig1 <> sig2}
+}.
+
+Structure F (sigT:Sig): Type := mkF {
+  F_carrier :> Type;
+  F_sig: forall (f:F_carrier), sigT
+}.
+
+Structure EF (sigT:Sig): Type := mkEF {
+  EF_carrier :> Type;
+  EF_dec: forall (ef1 ef2:EF_carrier), {ef1 = ef2} + {ef1 <> ef2};
+  EF_linkable: forall (ef:EF_carrier), bool;
+  EF_sig: forall (ef:EF_carrier), sigT
+}.
+
+Structure Fundef (sigT:Sig) (fT:F sigT) (efT:EF sigT) := mkFundef {
+  Fundef_carrier :> Type;
+  Fundef_dec: forall (fd:Fundef_carrier), fT + efT;
+  Fundef_sig :=
+    fun fd =>
+      match Fundef_dec fd with
+        | inl f => fT.(F_sig) f
+        | inr ef => efT.(EF_sig) ef
+      end
+}.
+
+Structure V: Type := mkV {
+  V_carrier :> Type;
+  V_dec: forall (v1 v2:V_carrier), {v1 = v2} + {v1 <> v2}
+}.
+
+Structure Language: Type := mkLanguage {
+  sigT: Sig;
+  fT: F sigT;
+  efT: EF sigT;
+  fundefT: Fundef fT efT;
+  vT: V;
+  globdefT := AST.globdef fundefT vT;
+  progT := AST.program fundefT vT
+}.
+
+Structure Language_ext: Type := mkLanguage_ext {
+  lang :> Language;
+
+  stateT: Type;
+  contT: Type;
+  mkCallstate: forall (cont:contT) (fd:lang.(fundefT)) (args:list val) (m:mem), stateT;
+  mkReturnstate: forall (cont:contT) (v:val) (m:mem), stateT;
+  empty_cont: contT;
+
+  step: forall (ge:Genv.t lang.(fundefT) lang.(vT)) (state1:stateT) (evt:Events.trace) (state2:stateT), Prop;
+  signature_main: lang.(sigT);
+  initial_state := fun (p:lang.(progT)) (state:stateT) =>
+                     exists b f m0,
+                       let ge := Genv.globalenv p in
+                       Genv.init_mem p = Some m0 /\
+                       Genv.find_symbol ge p.(prog_main) = Some b /\
+                       Genv.find_funct_ptr ge b = Some f /\
+                       lang.(fundefT).(Fundef_sig) f = signature_main /\
+                       state = (mkCallstate empty_cont f nil m0);
+  final_state := fun (state:stateT) (r:int) =>
+                   exists m,
+                     state = mkReturnstate empty_cont (Vint r) m;
+  semantics := fun (p:lang.(progT)) =>
+                 Semantics step (initial_state p) final_state (Genv.globalenv p);
+
+  Hfinal_not_progress: forall v m,
+                         ~ exists ge evt state', step ge (mkReturnstate empty_cont v m) evt state';
+  Hfinal_not_call: forall v m1,
+                     ~ exists cont fd args m2, mkReturnstate empty_cont v m1 = mkCallstate cont fd args m2;
+  HmkReturnstate_inj: forall cont1 v1 m1 cont2 v2 m2 (H: mkReturnstate cont1 v1 m1 = mkReturnstate cont2 v2 m2),
+                        cont1 = cont2 /\ v1 = v2 /\ m1 = m2
+}.
+
+(* Inductive initial_state (lang:Language_ext) (p:lang.(progT)): lang.(stateT) -> Prop := *)
+(*   | initial_state_intro: forall b f m0, *)
+(*       let ge := Genv.globalenv p in *)
+(*       Genv.init_mem p = Some m0 -> *)
+(*       Genv.find_symbol ge p.(prog_main) = Some b -> *)
+(*       Genv.find_funct_ptr ge b = Some f -> *)
+(*       lang.(fundefT).(Fundef_sig) f = lang.(signature_main) -> *)
+(*       initial_state lang p (lang.(mkCallstate) lang.(empty_cont) f nil m0). *)
+
+(* Inductive final_state (lang:Language_ext): lang.(stateT) -> int -> Prop := *)
+(*   | final_state_intro: forall r m, *)
+(*       final_state lang (lang.(mkReturnstate) lang.(empty_cont) (Vint r) m) r. *)
+
+(* Definition semantics (lang:Language_ext) (p:lang.(progT)) := *)
+(*   Semantics lang.(step) (initial_state lang p) (final_state lang) (Genv.globalenv p). *)
+
+(** Canonical Structures *)
+
+Canonical Structure Sig_type: Sig := mkSig Ctypes.type_eq.
+Canonical Structure Sig_signature: Sig := mkSig signature_eq.
+
+Canonical Structure F_C: F Sig_type := mkF Sig_type Csyntax.type_of_function.
+Canonical Structure F_Clight: F Sig_type := mkF Sig_type Clight.type_of_function.
+Canonical Structure F_Csharpminor: F Sig_signature := mkF Sig_signature Csharpminor.fn_sig.
+Canonical Structure F_Cminor: F Sig_signature := mkF Sig_signature Cminor.fn_sig.
+Canonical Structure F_CminorSel: F Sig_signature := mkF Sig_signature CminorSel.fn_sig.
+Canonical Structure F_RTL: F Sig_signature := mkF Sig_signature RTL.fn_sig.
+Canonical Structure F_LTL: F Sig_signature := mkF Sig_signature LTL.fn_sig.
+Canonical Structure F_Linear: F Sig_signature := mkF Sig_signature Linear.fn_sig.
+Canonical Structure F_Mach: F Sig_signature := mkF Sig_signature Mach.fn_sig.
+Canonical Structure F_Asm: F Sig_signature := mkF Sig_signature Asm.fn_sig.
+
+Canonical Structure EF_external_function_ext: EF Sig_type :=
+  mkEF Sig_type
+       external_function_ext_eq
+       (fun ef => match ef with (EF_external _ _, _, _, _) => true | _ => false end)
+       (fun ef => match ef with (_, targs, tres, cc) => Ctypes.Tfunction targs tres cc end).
+Canonical Structure EF_external_function: EF Sig_signature :=
+  mkEF Sig_signature
+       external_function_eq
+       (fun ef => match ef with EF_external _ _ => true | _ => false end)
+       ef_sig.
+
+Canonical Structure Fundef_C: Fundef F_C EF_external_function_ext :=
+  mkFundef F_C EF_external_function_ext
+           (fun fd =>
+              match fd with
+                | Csyntax.Internal f => inl f
+                | Csyntax.External ef targs tres cc => inr (ef, targs, tres, cc)
+              end).
+Canonical Structure Fundef_Clight: Fundef F_Clight EF_external_function_ext :=
+  mkFundef F_Clight EF_external_function_ext
+           (fun fd =>
+              match fd with
+                | Clight.Internal f => inl f
+                | Clight.External ef targs tres cc => inr (ef, targs, tres, cc)
+              end).
+Canonical Structure Fundef_common (fT:F Sig_signature): Fundef fT EF_external_function :=
+  mkFundef fT EF_external_function
+           (fun fd =>
+              match fd with
+                | AST.Internal f => inl f
+                | AST.External ef => inr ef
+              end).
+
+Canonical Structure V_type: V := mkV Ctypes.type_eq.
+Canonical Structure V_unit: V := mkV unit_eq.
+
+Canonical Structure Language_C: Language := mkLanguage Fundef_C V_type.
+Program Canonical Structure Language_ext_C: Language_ext :=
+  @mkLanguage_ext Language_C _ _
+                  (fun k fd args m => Csem.Callstate fd args k m)
+                  (fun k v m => Csem.Returnstate v k m)
+                  Csem.Kstop
+                  Csem.step
+                  (Ctypes.Tfunction Ctypes.Tnil Ctypes.type_int32s cc_default) _ _ _.
+Next Obligation. intros [ge [evt [state' Hstep]]]. inv Hstep. inv H. inv H. Qed.
+Canonical Structure Language_Clight: Language := mkLanguage Fundef_Clight V_type.
+Program Canonical Structure Language_ext_Clight1: Language_ext :=
+  @mkLanguage_ext Language_Clight _ _
+                  (fun k fd args m => Clight.Callstate fd args k m)
+                  (fun k v m => Clight.Returnstate v k m)
+                  Clight.Kstop
+                  Clight.step1
+                  (Ctypes.Tfunction Ctypes.Tnil Ctypes.type_int32s cc_default) _ _ _.
+Next Obligation. intros [ge [evt [state' Hstep]]]. inv Hstep. Qed.
+Program Canonical Structure Language_ext_Clight2: Language_ext :=
+  @mkLanguage_ext Language_Clight _ _
+                  (fun k fd args m => Clight.Callstate fd args k m)
+                  (fun k v m => Clight.Returnstate v k m)
+                  Clight.Kstop
+                  Clight.step2
+                  (Ctypes.Tfunction Ctypes.Tnil Ctypes.type_int32s cc_default) _ _ _.
+Next Obligation. intros [ge [evt [state' Hstep]]]. inv Hstep. Qed.
+Canonical Structure Language_Csharpminor: Language := mkLanguage (Fundef_common F_Csharpminor) V_unit.
+Program Canonical Structure Language_ext_Csharpminor: Language_ext :=
+  @mkLanguage_ext Language_Csharpminor _ _
+                  (fun k fd args m => Csharpminor.Callstate fd args k m)
+                  (fun k v m => Csharpminor.Returnstate v k m)
+                  Csharpminor.Kstop
+                  Csharpminor.step
+                  AST.signature_main _ _ _.
+Next Obligation. intros [ge [evt [state' Hstep]]]. inv Hstep. Qed.
+Canonical Structure Language_Cminor: Language := mkLanguage (Fundef_common F_Cminor) V_unit.
+Program Canonical Structure Language_ext_Cminor: Language_ext :=
+  @mkLanguage_ext Language_Cminor _ _
+                  (fun k fd args m => Cminor.Callstate fd args k m)
+                  (fun k v m => Cminor.Returnstate v k m)
+                  Cminor.Kstop
+                  Cminor.step
+                  AST.signature_main _ _ _.
+Next Obligation. intros [ge [evt [state' Hstep]]]. inv Hstep. Qed.
+Canonical Structure Language_CminorSel: Language := mkLanguage (Fundef_common F_CminorSel) V_unit.
+Program Canonical Structure Language_ext_CminorSel: Language_ext :=
+  @mkLanguage_ext Language_CminorSel _ _
+                  (fun k fd args m => CminorSel.Callstate fd args k m)
+                  (fun k v m => CminorSel.Returnstate v k m)
+                  CminorSel.Kstop
+                  CminorSel.step
+                  AST.signature_main _ _ _.
+Next Obligation. intros [ge [evt [state' Hstep]]]. inv Hstep. Qed.
+Canonical Structure Language_RTL: Language := mkLanguage (Fundef_common F_RTL) V_unit.
+Program Canonical Structure Language_ext_RTL: Language_ext :=
+  @mkLanguage_ext Language_RTL _ _
+                  RTL.Callstate
+                  RTL.Returnstate
+                  nil
+                  RTL.step
+                  AST.signature_main _ _ _.
+Next Obligation. intros [ge [evt [state' Hstep]]]. inv Hstep. Qed.
+Canonical Structure Language_LTL: Language := mkLanguage (Fundef_common F_LTL) V_unit.
+Canonical Structure Language_Linear: Language := mkLanguage (Fundef_common F_Linear) V_unit.
+Canonical Structure Language_Mach: Language := mkLanguage (Fundef_common F_Mach) V_unit.
+Canonical Structure Language_Asm: Language := mkLanguage (Fundef_common F_Asm) V_unit.
