common/ProgramLSim.v
@@ -3,7 +3,7 @@ Require String.
 Require Import Coqlib Coqlib_linker.
 Require Import Maps Maps_linker.
 Require Import Integers Floats Values AST Globalenvs.
-Require Import LinkerSpecification LinkerProp Linkeq.
+Require Import Language Linker LinkerProp Linkeq.
 Require Import Errors.
 Require Import paco.
 
